theories/proofmode/reduction.v
@@ -12,7 +12,7 @@ Declare Reduction pm_eval := cbv [
   env_dom env_intuitionistic env_spatial env_counter env_spatial_is_nil envs_dom
   envs_lookup envs_lookup_delete envs_delete envs_snoc envs_app
   envs_simple_replace envs_replace envs_split
-  envs_clear_spatial envs_clear_persistent envs_incr_counter
+  envs_clear_spatial envs_clear_intuitionistic envs_incr_counter
   envs_split_go envs_split env_to_prop
   (* PM option combinators *)
   pm_option_bind pm_from_option pm_option_fun
